hinata_mikami/gc/output/gc/proofs/proof_Heap_alloc.v
@@ -1,35 +1,13 @@
 From caesium Require Import lang notation.
 From refinedrust Require Import typing shims.
 From refinedrust.examples.gc.generated Require Import generated_code_gc generated_specs_gc generated_template_Heap_alloc.
-
-(* 不要 *)
-(* From hinata_mikami.extra_proofs.gc Require Import heap_lemmas. *)
+From hinata_mikami.extra_proofs.gc Require Import heap_lemmas.
 
 Set Default Proof Using "Type".
 
 Section proof.
 Context `{RRGS : !refinedrustGS Σ}.
 
-(* 
-Lemma simplify_goal_big_sepL_app {A}
-    (xs1 xs2 : list A)
-    (Φ : nat → A → iProp Σ) T :
-  ([∗ list] i ↦ x ∈ xs1, Φ i x) ∗
-  ([∗ list] i ↦ x ∈ xs2,
-      Φ (length xs1 + i)%nat x) ∗ T
-  ⊢
-  simplify_goal
-    ([∗ list] i ↦ x ∈ xs1 ++ xs2, Φ i x) T.
-Proof.
-  rewrite /simplify_goal.
-  rewrite big_sepL_app.
-  iIntros "($ & $ & $)".
-Qed.
-
-Definition simplify_goal_big_sepL_app_inst :=
-  [instance @simplify_goal_big_sepL_app with 10%N].
-
-Global Existing Instance simplify_goal_big_sepL_app_inst. *)
 
 (* hinata_mikami.extra_proofs.gc で定義したものが認識されているか確認 *)
 (* Check simplify_goal_big_sepL_app.
@@ -232,7 +210,187 @@ Proof.
     iRename select
       (freeable_nz x' _ _ _)
       into "Hfree_new".
-      
+    
+        (* -------------------------------------------------- *)
+    (* Node のサイズが正であること                       *)
+    (* -------------------------------------------------- *)
+
+    assert (Hvalue_field :
+      ("value", IntSynType I32) ∈ Node_sls.(sls_fields)).
+    {
+      rewrite /Node_sls /=.
+      set_solver.
+    }
+
+    destruct
+      (struct_layout_spec_has_layout_members
+        Node_sls Node_sl
+        "value" (IntSynType I32)
+        H9 Hvalue_field)
+      as (value_ly & Hvalue_mem & Hvalue_layout).
+
+    apply syn_type_has_layout_int_inv in Hvalue_layout.
+    subst value_ly.
+
+    assert (Hsize_mem :
+      ly_size (it_layout I32) ∈
+        (ly_size <$> (sl_members Node_sl).*2)).
+    {
+      apply (list_elem_of_fmap_2 ly_size).
+
+      apply
+        (list_elem_of_fmap_2
+          snd
+          (sl_members Node_sl)
+          (Some "value", it_layout I32)).
+
+      exact Hvalue_mem.
+    }
+
+    pose proof
+      (sum_list_with_in
+        (ly_size (it_layout I32))
+        id
+        (ly_size <$> (sl_members Node_sl).*2)
+        Hsize_mem)
+      as Hsize_le.
+
+    assert (HNode_sl_pos :
+      (0 < ly_size Node_sl)%nat).
+    {
+      rewrite /ly_size /layout_of /=.
+
+      assert (Hval_pos :
+        (0 < ly_size (it_layout I32))%nat).
+      {
+        rewrite /it_layout /ly_size /bytes_per_int /it_byte_size_log.
+        simpl.
+        lia.
+      }
+
+      change (0 < bytes_per_int I32)%nat in Hval_pos.
+
+      eapply Nat.lt_le_trans.
+      - exact Hval_pos.
+      - exact Hsize_le.
+    }
+
+    assert (HNode_alg :
+      use_layout_alg Node_sls =
+        Some (layout_of Node_sl)).
+    {
+      apply use_struct_layout_alg_Some_inv.
+      exact H9.
+    }
+
+    assert (Hnode_size_pos :
+      (0 < ly_size (use_layout_alg' Node_sls))%nat).
+    {
+      rewrite /use_layout_alg'.
+      rewrite HNode_alg.
+      simpl.
+      exact HNode_sl_pos.
+    }
+
+    destruct (decide (x' ∈ old_l :: locs_tail))
+      as [Hin_old | Hfresh].
+    {
+      rewrite elem_of_cons in Hin_old.
+      destruct Hin_old as [Hx_head | Hx_tail].
+
+      (* x' = old_l の場合 *)
+      {
+        iDestruct "Hfirst" as
+          (l n m)
+          "(%Heq_l & %Heq_n & %Heq_m &
+            Hguard_first & Hfree_first)".
+
+        injection Heq_l as Heq_l.
+        subst l.
+
+        iDestruct
+          (freeable_nz_full_ne
+            x' old_l
+            (ly_size (use_layout_alg' Node_sls))
+            HeapAlloc HeapAlloc
+            Hnode_size_pos
+            with "Hfree_new Hfree_first")
+          as %Hne.
+
+        iExFalso.
+        iPureIntro.
+        exact (Hne Hx_head).
+      }
+
+      (* x' が locs_tail のどこかにある場合 *)
+      {
+        destruct
+          (list_elem_of_lookup_1 locs_tail x' Hx_tail)
+          as [i Hloc_x].
+
+        pose proof
+          (lookup_lt_Some _ _ _ Hloc_x)
+          as Hi_locs.
+
+        assert (Hi_vals :
+          (i < length vals_tail)%nat).
+        {
+          rewrite -Hlen_locs_tail.
+          exact Hi_locs.
+        }
+
+        destruct
+          (lookup_lt_is_Some_2 vals_tail i)
+          as [vi Hvi].
+        {
+          exact Hi_vals.
+        }
+
+        iDestruct
+          (big_sepL_lookup_acc with "Htail_ext")
+          as "[HiNode Hclose]".
+        {
+          exact Hvi.
+        }
+
+        iDestruct "HiNode" as
+          (l n m)
+          "(%Hloc_ext & %Hnext_ext & %Hmark_ext &
+            Hguard_old & Hfree_old)".
+
+        rewrite lookup_app_l in Hloc_ext;
+          last exact Hi_locs.
+
+        assert (l = x') as Heq_l.
+        {
+          congruence.
+        }
+        subst l.
+
+        iDestruct
+          (freeable_nz_full_ne
+            x' x'
+            (ly_size (use_layout_alg' Node_sls))
+            HeapAlloc HeapAlloc
+            Hnode_size_pos
+            with "Hfree_new Hfree_old")
+          as %Hne.
+
+        iExFalso.
+        iPureIntro.
+        exact (Hne eq_refl).
+      }
+    }
+
+    assert (Hnodup_new :
+      NoDup ((old_l :: locs_tail) ++ [x'])).
+    {
+      apply NoDup_snoc_local.
+      - exact Hnodup_locs.
+      - exact Hfresh.
+    }
+
+    (* --- *)
     assert (Hlen_nexts_new :
       S (length (nexts_tail ++ [NULL_loc])) =
       S (length (vals_tail ++ [v]))).
@@ -398,9 +556,8 @@ Proof.
     - set_solver.
     - constructor.
   }
-  {
-    
-  }
+  
+
   Unshelve.
   all: print_remaining_sidecond.
 Qed.
